proof/spec/KyberProperties.ec
@@ -3,6 +3,7 @@ from Jasmin require import JWord.
 require import Array32 Array64 Array128 Array168 Array256 Array384.
 require import Array768 Array960 Array1024 Array1152.
 require import Kyber.
+require import EncDecCorrectness.
 import NTT_Properties.
 (* Aux *)
 import KMatrix.
@@ -30,6 +31,38 @@ apply Array256.tP => k kb.
 by rewrite mapiE //= initiE //= mapiE 1:/# initiE 1:/# /= asintK /#.
 qed.
 
+
+(* These are a pain but need to be done. See EncDecCorrectness. *) 
+lemma sem_encode1K (x : ipoly) : 
+   (forall i, 0 <= i < 256 => 0 <= x.[i] < 2) =>
+     x = (op_EncDec_decode1 (op_EncDec_encode1 x)) by admit.
+lemma sem_encode4K (x : ipoly) : 
+   (forall i, 0 <= i < 256 => 0 <= x.[i] < 16) =>
+     x =  op_EncDec_decode4 (op_EncDec_encode4 x)  by admit. 
+lemma sem_encode10_vecK (x : ipolyvec) : 
+   (forall i, 0 <= i < 768 => 0 <= x.[i] < 1024) =>
+     x =  op_EncDec_decode10_vec (op_EncDec_encode10_vec x)  by admit. 
+lemma sem_encode12_vecK (x : ipolyvec) : 
+   (forall i, 0 <= i < 768 => 0 <= x.[i] < 4096) =>
+     x =  op_EncDec_decode12_vec (op_EncDec_encode12_vec x)  by admit. 
+
+require import BitEncoding.  
+import BS2Int BitChunking.
+lemma sem_decode1_bnd a k : 0<=k<256 => 0<= (sem_decode1 a).[k] < 2.
+proof.
+move => kb; rewrite /sem_decode1 get_of_list //. 
+pose ll := decode _ _.
+have Hs : size ll = 256 by
+  rewrite /ll /decode size_map size_chunk //= size_take_le //=; 
+  smt(Array32.size_to_list size_BytesToBits).
+have /= := (all_nthP (fun (b : int) => 0<= b < 2) ll 0) .
+have ->  /= : all (fun (b : int) => 0 <= b && b < 2) ll; last by smt().
+rewrite allP /ll /decode => /= i.
+rewrite mapP => Hm; elim Hm => v [Hv ->].
+have Hsv := (in_chunk_size _ _ _ _ Hv); 1: smt().
+have := bs2int_range v; rewrite Hsv /=.
+by smt(mem_range).
+qed.
 
 (**************************************************************************
    MLWE_PKE is the theory where we prove an abstract PKE construction
@@ -60,14 +93,14 @@ type pkey = W8.t Array1152.t * W8.t Array32.t.
 type skey = W8.t Array1152.t.  
 
 op pk_encode(pk : vector * W8.t Array32.t) : pkey = 
-                                  (sem_encode12_vec (toipolyvec (nttv pk.`1)) ,pk.`2).
+                                  (op_EncDec_encode12_vec (toipolyvec (nttv pk.`1)) ,pk.`2).
 op pk_decode(pk : pkey) = (invnttv (ofipolyvec (sem_decode12_vec (pk.`1))),pk.`2).
-op sk_encode(sk : vector) : skey = sem_encode12_vec (toipolyvec (nttv sk)).
+op sk_encode(sk : vector) : skey = op_EncDec_encode12_vec (toipolyvec (nttv sk)).
 op sk_decode(sk : skey) =  invnttv (ofipolyvec (sem_decode12_vec sk)).
 op m_encode(m : plaintext) : poly = decompress_poly 1 (sem_decode1 m).
-op m_decode(p : poly) : plaintext = sem_encode1 (compress_poly 1 p). 
+op m_decode(p : poly) : plaintext = op_EncDec_encode1 (compress_poly 1 p). 
 op c_encode(c :  vector * poly) : ciphertext = 
-      (sem_encode10_vec (compress_polyvec 10 c.`1), sem_encode4 (compress_poly 4 c.`2)).
+      (op_EncDec_encode10_vec (compress_polyvec 10 c.`1), op_EncDec_encode4 (compress_poly 4 c.`2)).
 op c_decode(c : ciphertext) =
       (decompress_polyvec 10 (sem_decode10_vec c.`1), decompress_poly 4 (sem_decode4 c.`2)).
 op rnd_err_v = compress_poly_err 4. 
@@ -163,17 +196,24 @@ clone import MLWE_PKE as MLWEPKE with
 
 realize pk_encodeK.
 rewrite /pk_decode /pk_encode /cancel /= => x.
-by rewrite sem_encode12_vecK toipolyvecK invnttvK /#.
+rewrite sem_decode12_vec_corr -sem_encode12_vecK; last by rewrite toipolyvecK invnttvK /#.
+move => i ib; rewrite /toipolyvec !mapiE /= 1:ib.
+by smt(rg_asint qE).
 qed.
 
 realize sk_encodeK.
 rewrite /sk_decode /sk_encode /cancel /= => x.
-rewrite sem_encode12_vecK toipolyvecK invnttvK /#.
+rewrite sem_decode12_vec_corr  -sem_encode12_vecK; last by rewrite toipolyvecK invnttvK /#.
+move => i ib; rewrite /toipolyvec !mapiE /= 1:ib.
+by smt(rg_asint qE).
 qed.
 
 realize encode_noise.
 move => /> u v.
-rewrite /c_decode /c_encode /rnd_err_u /rnd_err_v /= sem_encode10_vecK sem_encode4K => />.
+rewrite /c_decode /c_encode /rnd_err_u /rnd_err_v /z sem_decode10_vec_corr /= -sem_encode10_vecK.
++ move => i ib; rewrite /compress_polyvec !mapiE /= 1:ib /compress /= /#.
+rewrite sem_decode4_corr -sem_encode4K /=.
++ move => i ib; rewrite /compress_poly !mapiE /= 1:ib /compress /= /#.
 split; last  by rewrite round_poly_errE.
 rewrite /(+) /mapv /=.
 apply eq_vectorP => /> i il ih; rewrite !offunvE 1,2:/# /=.
@@ -189,10 +229,14 @@ realize good_decode.
 rewrite /under_noise_bound /m_encode /m_decode /compress_poly 
         /decompress_poly /max_noise qE /= => m n.
 rewrite allP  => /=  hgood.
-have : sem_decode1 (sem_encode1 (map (compress 1) (map (decompress 1) (sem_decode1 m) &+ n))) = 
-       (sem_decode1 m); last by smt(sem_decode1K).
+rewrite sem_decode1_corr.
+have : op_EncDec_decode1 (op_EncDec_encode1 (map (compress 1) (map (decompress 1) (op_EncDec_decode1 m) &+ n))) = 
+       (op_EncDec_decode1 m); last by smt(sem_decode1K).
 apply Array256.ext_eq => /> x h0x hx256. 
-rewrite sem_encode1K /(&+) mapiE 1:/# map2E /= initiE /= 1:/# mapiE 1:/#.
+rewrite -sem_encode1K. 
++ move => i ib; rewrite !mapiE /= 1:ib /compress /= /#.
+rewrite /(&+) mapiE 1:/# map2E /= initiE /= 1:/# mapiE 1:/#.
+rewrite -sem_decode1_corr.
 have [->|->] /=: (sem_decode1 m).[x]=0 \/ (sem_decode1 m).[x]=1
  by smt(sem_decode1_bnd).
  rewrite /decompress /=.
@@ -844,6 +888,18 @@ module (NTTSampler(S : Sampler) : Sampler) (O : RO.POracle) = {
 
 }.
 
+(* These are all replaced by proc op *)
+phoare sem_decode1  a : [ EncDec.decode1  : arg = a ==>  res = op_EncDec_decode1  a ] = 1%r by admit. (* reify *)
+phoare sem_encode12 a : [ EncDec.encode12 : arg = a ==>  res = op_EncDec_encode12 a ] = 1%r by admit. (* reify *)
+phoare sem_encode1  a : [ EncDec.encode1  : arg = a ==>  res = op_EncDec_encode1  a ] = 1%r by admit. (* reify *)
+phoare sem_encode4  a : [ EncDec.encode4  : arg = a ==>  res = op_EncDec_encode4  a ] = 1%r by admit. (* reify *)
+phoare sem_decode4  a : [ EncDec.decode4  : arg = a ==>  res = op_EncDec_decode4  a ] = 1%r by admit. (* reify *)
+phoare sem_encode10_vec a : [ EncDec.encode10_vec : arg = a ==> res = op_EncDec_encode10_vec a ] = 1%r by admit. (* reify *)
+phoare sem_decode10_vec a : [ EncDec.decode10_vec : arg = a ==> res = op_EncDec_decode10_vec a ] = 1%r by admit. (* reify *)
+phoare sem_encode12_vec a : [ EncDec.encode12_vec : arg = a ==> res = op_EncDec_encode12_vec a ] = 1%r by admit. (* reify *)
+phoare sem_decode12_vec a : [ EncDec.decode12_vec : arg = a ==> res = op_EncDec_decode12_vec a ] = 1%r by admit. (* reify *)
+
+
 section.
 
 declare module O <: RO.Oracle {-IdealHSF.RF,-RF,-IdealPRF1.RF}.
@@ -1106,7 +1162,8 @@ wp;ecall{2}(sem_decode12_vec (tv{2})).
 auto => /> &1 &2; rewrite /pk_decode /c_encode /m_encode /=.  
 split; 1: by rewrite -comm_nttv_mmul invnttvK.
 congr. congr. congr. congr.
-by rewrite comm_ntt_dotp.
+by rewrite comm_ntt_dotp sem_decode12_vec_corr.
+by rewrite sem_decode1_corr.
 qed.
 
 equiv dec_eq : 
@@ -1121,7 +1178,8 @@ wp;ecall{2} (sem_decode10_vec (c1{2})).
 auto => /> &2.
 rewrite /m_decode /sk_decode /c_decode /=.
 congr. congr. congr. 
-by rewrite comm_ntt_dotp.
+by rewrite sem_decode4_corr.
+by rewrite comm_ntt_dotp sem_decode10_vec_corr sem_decode12_vec_corr.
 qed.
 
 end section.
